is_eval_once deterministic

formal/SkLean/Sn.lean
@@ -1,13 +1,12 @@
 import SkLean.Ast3
 
-inductive sn : Expr → Prop
-  | hard : (∀ e', is_eval_once e e' → sn e') → sn e
+def sn (e : Expr) := Acc (λ e' e => is_eval_once e e') e
 
 syntax (name := do_stuck) "do_stuck " : tactic
 
 macro_rules
   | `(tactic| do_stuck) =>
-    `(tactic| apply sn.hard; intro e h_step; contradiction)
+    `(tactic| apply Acc.intro; intro e h_step; contradiction)
 
 namespace sn
 
@@ -26,8 +25,8 @@ lemma m : sn SKM[M] := by
 lemma preserved : sn e → is_eval_once e e' → sn e' := by
   intro h_sn h_eval
   induction h_sn
-  case hard e ih₁ ih₂ =>
-    simp_all
+  case intro e ih₁ ih₂ =>
+    exact ih₁ _ h_eval
 
 end sn
 
@@ -36,43 +35,82 @@ lemma is_value_sn (h_v : is_value e) : sn e := by
   repeat do_stuck
 
 inductive is_candidate_for_ty : Expr → Expr → Prop
-  | val   : valid_judgment e t
+  | val : valid_judgment e t
     → is_value e
     → is_candidate_for_ty e t
-  | step  : valid_judgment e t
-    → is_candidate_for_ty e t
-    → is_eval_once e e'
-    → is_candidate_for_ty e' t
-  | stuck : valid_judgment e t
-    → (∀ e', is_eval_once e e' → is_candidate_for_ty e' t)
-    → is_candidate_for_ty e t
+  | app : is_candidate_for_ty lhs SKM[(t_in ~> t_out)]
+    → is_candidate_for_ty rhs t_in
+    → is_eval_once SKM[(lhs rhs)] e'
+    → is_candidate_for_ty e' t_out
+    → is_candidate_for_ty SKM[(lhs rhs)] t_out
 
 namespace is_candidate_for_ty
 
+lemma all_well_typed (h : is_candidate_for_ty e t) : valid_judgment e t := by
+  induction h
+  repeat assumption
+  apply valid_judgment.call
+  repeat assumption
+
 lemma all_sn (h_candidate : is_candidate_for_ty e t) : sn e := by
   induction h_candidate
-  exact is_value_sn (by assumption)
-  exact sn.preserved (by assumption) (by assumption)
-  case stuck e' t' h_t_e ih₁ ih₂ =>
-    have h_t'' := h_t_e.progress
-    match h_t'' with
-      | .inl h_stuck =>
-        exact is_value_sn (by assumption)
-      | .inr ⟨t, h_step⟩ =>
-        apply sn.hard
-        simp_all
+  case val h =>
+    exact is_value_sn (by assumption)
+  case app lhs t_in t_out rhs e' h_t_lhs h_t_rhs h_step ih₁ ih₂ ih₃ =>
+    apply Acc.intro
+    intro e' h_step'
+    cases ih₃
+    
+    sorry
 
-lemma all_well_typed (h_candidate : is_candidate_for_ty e t) : valid_judgment_hard e t := by
-  induction h_candidate
+lemma valid_call (h_candidate_lhs : is_candidate_for_ty lhs SKM[(t_in ~> t_out)]) (h_candidate_rhs : is_candidate_for_ty rhs t_in) : is_candidate_for_ty SKM[(lhs rhs)] t_out := by
+  cases h_candidate_lhs
+  apply is_candidate_for_ty.stuck
+  apply valid_judgment.call
   assumption
-  apply valid_judgment.preservation
+  exact h_candidate_rhs.all_well_typed
+  intro e' h_step
+  have h_t : valid_judgment SKM[(lhs rhs)] t_out := by
+    sorry
+  have h_t' := h_t.preservation h_step
+  apply is_candidate_for_ty.step
+  exact h_t'
   
+  sorry
 
 end is_candidate_for_ty
 
 namespace valid_judgment
 
+lemma all_candidates (h_t : valid_judgment e t) : is_candidate_for_ty e t := by
+  induction h_t
+  sorry
+  sorry
+  sorry
+  sorry
+  sorry
+  sorry
+  sorry
+  sorry
+  sorry
+  sorry
+  sorry
+  case call lhs t_in t_out rhs h_t_lhs h_t_rh sih₁ ih₂ =>
+    
+    sorry
 
+end valid_judgment
+
+namespace valid_judgment
+
+theorem sn (h_t : valid_judgment e t) : sn e := by
+  let h_t₀ := h_t
+  induction h_t
+  repeat do_stuck
+  case call lhs t_in t_out rhs h_t_lhs h_t_rhs ih₁ ih₂ =>
+    let e' := h_t₀.progress
+    
+    sorry
 
 end valid_judgment
 
